CoqOfRust/plonky3/keccak_air/links/constants.v
@@ -1,0 +1,138 @@
+Require Import CoqOfRust.CoqOfRust.
+Require Import CoqOfRust.links.M.
+Require Import core.links.array.
+Require Import plonky3.keccak_air.constants.
+
+(*
+pub(crate) const R: [[u8; 5]; 5] = [
+    [0, 36, 3, 41, 18],
+    [1, 44, 10, 45, 2],
+    [62, 6, 43, 15, 61],
+    [28, 55, 25, 21, 56],
+    [27, 20, 39, 8, 14],
+];
+*)
+Definition R : array.t (array.t U8.t {| Integer.value := 5 |}) {| Integer.value := 5 |} :=
+  {|
+    array.value := [
+      {| array.value := List.map (Integer.Build_t IntegerKind.U8) [0; 36; 3; 41; 18] |};
+      {| array.value := List.map (Integer.Build_t IntegerKind.U8) [1; 44; 10; 45; 2] |};
+      {| array.value := List.map (Integer.Build_t IntegerKind.U8) [62; 6; 43; 15; 61] |};
+      {| array.value := List.map (Integer.Build_t IntegerKind.U8) [28; 55; 25; 21; 56] |};
+      {| array.value := List.map (Integer.Build_t IntegerKind.U8) [27; 20; 39; 8; 14] |}
+    ]
+  |}.
+
+Instance run_value_R :
+  Run.Trait constants.value_R [] [] []
+    (Ref.t Pointer.Kind.Raw (array.t (array.t U8.t {| Integer.value := 5 |}) {| Integer.value := 5 |})).
+Proof.
+  constructor.
+  run_symbolic.
+Defined.
+
+(*
+pub const RC: [u64; 24] = [
+    0x0000000000000001,
+    0x0000000000008082,
+    0x800000000000808A,
+    0x8000000080008000,
+    0x000000000000808B,
+    0x0000000080000001,
+    0x8000000080008081,
+    0x8000000000008009,
+    0x000000000000008A,
+    0x0000000000000088,
+    0x0000000080008009,
+    0x000000008000000A,
+    0x000000008000808B,
+    0x800000000000008B,
+    0x8000000000008089,
+    0x8000000000008003,
+    0x8000000000008002,
+    0x8000000000000080,
+    0x000000000000800A,
+    0x800000008000000A,
+    0x8000000080008081,
+    0x8000000000008080,
+    0x0000000080000001,
+    0x8000000080008008,
+];
+*)
+Definition RC : array.t U64.t {| Integer.value := 24 |} :=
+  {|
+    array.value := List.map (Integer.Build_t IntegerKind.U64) [
+      0x0000000000000001;
+      0x0000000000008082;
+      0x800000000000808A;
+      0x8000000080008000;
+      0x000000000000808B;
+      0x0000000080000001;
+      0x8000000080008081;
+      0x8000000000008009;
+      0x000000000000008A;
+      0x0000000000000088;
+      0x0000000080008009;
+      0x000000008000000A;
+      0x000000008000808B;
+      0x800000000000008B;
+      0x8000000000008089;
+      0x8000000000008003;
+      0x8000000000008002;
+      0x8000000000000080;
+      0x000000000000800A;
+      0x800000008000000A;
+      0x8000000080008081;
+      0x8000000000008080;
+      0x0000000080000001;
+      0x8000000080008008
+    ]
+  |}.
+
+Instance run_value_RC :
+  Run.Trait constants.value_RC [] [] []
+    (Ref.t Pointer.Kind.Raw (array.t U64.t {| Integer.value := 24 |})).
+Proof.
+  constructor.
+  unshelve eapply Run.CallPrimitiveStateAlloc. {
+    eapply OfValue.Make with (value := RC).
+    reflexivity.
+  }
+  cbn; intros.
+  run_symbolic.
+Defined.
+
+(* const RC_BITS: [[u8; 64]; 24] *)
+Definition RC_BITS : array.t (array.t U8.t {| Integer.value := 64 |}) {| Integer.value := 24 |} :=
+  {|
+    array.value :=
+      List.map
+        (fun x => {|
+          array.value :=
+            List.map
+              (fun i => {| Integer.value := Z.b2z (Z.testbit x.(Integer.value) (Z.of_nat i)) |})
+              (List.seq 0 64)
+        |})
+        RC.(array.value)
+  |}.
+
+Instance run_value_RC_BITS :
+  Run.Trait constants.value_RC_BITS [] [] []
+    (Ref.t Pointer.Kind.Raw (array.t (array.t U8.t {| Integer.value := 64 |}) {| Integer.value := 24 |})).
+Proof.
+  constructor.
+  unshelve eapply Run.CallPrimitiveStateAlloc. {
+    eapply OfValue.Make with (value := RC_BITS).
+    reflexivity.
+  }
+  cbn; intros.
+  run_symbolic.
+Defined.
+
+(* pub(crate) const fn rc_value_bit(round: usize, bit_index: usize) -> u8 *)
+Instance run_value_rc_value_bit (round bit_index : Usize.t) :
+  Run.Trait constants.rc_value_bit [] [] [ φ round; φ bit_index ] U8.t.
+Proof.
+  constructor.
+  run_symbolic.
+Defined.
