CoqOfRust/plonky3/keccak_air/links/round_flags.v
@@ -1,0 +1,19 @@
+Require Import CoqOfRust.CoqOfRust.
+Require Import CoqOfRust.links.M.
+Require Import plonky3.air.links.air.
+Require Import plonky3.keccak_air.round_flags.
+
+(* pub(crate) fn eval_round_flags<AB: AirBuilder>(builder: &mut AB) *)
+Instance run_eval_round_flags
+    {AB : Set} `{Link AB}
+    `{run_AirBuilder_for_AB : AirBuilder.Run AB}
+    (builder : Ref.t Pointer.Kind.MutRef AB) :
+  Run.Trait round_flags.eval_round_flags
+    [] [Φ AB] [φ builder]
+    unit.
+Proof.
+  constructor.
+  run_symbolic_one_step.
+  run_symbolic_one_step.
+  run_symbolic_one_step.
+Admitted.
